tweaks to cloning

common/bindings.ec
@@ -1,17 +1,13 @@
 require import AllCore List IntDiv QFABV.
 
 from Jasmin require import JModel_x86.
-
-from JazzEC require import Array4 Array5 Array6 Array7 Array8 Array9 Array24 Array25 Array32.
-from JazzEC require import Array48 Array50 Array256 Array768 Array960.
-from JazzEC require import WArray32 WArray512 WArray960 WArray1536.
+from JazzEC require import Array4 Array5 Array6 Array7 Array8 Array9 Array16 Array24 Array25 Array32 Array48 Array128 Array160 Array256 Array384 Array768 Array960 Array1088 Array1024 Array1152 Array1408 Array1536 WArray1568 Array1410 Array1 Array2.
+from JazzEC require import WArray16 WArray32 WArray128 WArray160 WArray512 WArray960 WArray2048 WArray1536 Array1568 WArray1410 WArray384 WArray1088.
 
 import BitEncoding BS2Int BitChunking.
 
 require import JWord_extra.
 
-
-(* TO BE MOVED! *)
 
 (*[size_flatten] (for uniform inner lists) *)
 lemma size_flatten' ['a] sz (ss: 'a list list):
@@ -26,13 +22,29 @@ rewrite -(StdBigop.Bigint.BIA.eq_big_seq (fun _ => sz)) /=.
 by rewrite StdBigop.Bigint.big_constz count_predT.
 qed.
 
-
-(* END MOVED *)
-
+lemma flatten_ctt_inj ['a] (n : int) (s s' : 'a list list):
+     0 < n =>
+     (forall (x : 'a list), x \in s => size x = n) =>
+     (forall (x : 'a list), x \in s' => size x = n) =>
+     flatten s = flatten s' <=> s = s'.
+move=> Hn H1 H2; split; last by auto.
+move => Hf.
+have ? : size s = size s'.
++ have ? := size_flatten_ctt n s _;1:smt().
+  have ? := size_flatten_ctt n s' _;1:smt().
+  have ? : n * size s' = n * size s by smt().
+  by smt().
+apply (eq_from_nth []); 1:smt().
+move => i ib.
+apply (eq_from_nth witness);1:smt(mem_nth).
+move => ii iib.
+have -> : nth witness (nth [] s i) ii  = nth witness (flatten s) (i * n + ii) by rewrite (nth_flatten witness n);smt(@List).
+have -> : nth witness (nth [] s' i) ii  = nth witness (flatten s') (i * n + ii) by rewrite (nth_flatten witness n);smt(@List).
+by smt().
+qed.
 
 
 (* ----------- BEGIN BOOL BINDINGS ---------- *)
-import Bool.
 op bool2bits (b : bool) : bool list = [b].
 op bits2bool (b: bool list) : bool = List.nth false b 0.
 
@@ -50,14 +62,60 @@ realize tosintP by move => bv => //.
 bind op bool (/\) "and".
 realize bvandP by move=> bv1 bv2; rewrite /bool2bits /#.
 
-bind op bool (\/) "or".
-realize bvorP by move=> bv1 bv2; rewrite /bool2bits /#.
 
-bind op bool (^^) "xor".
-realize bvxorP by move=> bv1 bv2; rewrite /bool2bits /#.
+(* ----------- BEGIN W4 BINDINGS ---------- *)
 
-bind op bool [!] "not".
-realize bvnotP by move=> bv1; rewrite /bool2bits /#.
+theory W4.
+abbrev [-printing] size = 4.
+clone include BitWordSH with op size <- size
+rename "_XX" as "_4"
+proof gt0_size by done,
+size_le_256 by done.
+
+end W4. export W4 W4.ALU W4.SHIFT.
+
+bind bitstring W4.w2bits W4.bits2w W4.to_uint W4.to_sint W4.of_int W4.t 4.
+realize size_tolist by auto.
+realize tolistP by auto.
+realize oflistP by smt(W4.bits2wK). 
+realize ofintP by move => *;rewrite /of_int int2bs_mod.
+realize tosintP. move => bv /=;rewrite /to_sint /smod /= /BVA_Top_W4_t.msb.
+have -> /=: nth false (w2bits bv) (4 - 1) = 2 ^ (4 - 1) <= to_uint bv; last by smt().
+rewrite /to_uint. 
+rewrite -{2}(cat_take_drop 3 (w2bits bv)).
+rewrite bs2int_cat size_take 1:// W4.size_w2bits /=.
+rewrite -bs2int_div 1:// /= get_to_uint /=.
+rewrite -bs2int_mod 1:// /= /to_uint.
+by smt(bs2int_range mem_range W4.size_w2bits pow2_4).
+qed.
+realize touintP by smt().
+
+(* ----------- BEGIN W5 BINDINGS ---------- *)
+
+theory W5.
+abbrev [-printing] size = 5.
+clone include BitWordSH with op size <- size
+rename "_XX" as "_5"
+proof gt0_size by done,
+size_le_256 by done.
+
+end W5. export W5 W5.ALU W5.SHIFT.
+
+bind bitstring W5.w2bits W5.bits2w W5.to_uint W5.to_sint W5.of_int W5.t 5.
+realize size_tolist by auto.
+realize tolistP by auto.
+realize oflistP by smt(W5.bits2wK). 
+realize ofintP by move => *;rewrite /of_int int2bs_mod.
+realize tosintP. move => bv /=;rewrite /to_sint /smod /= /BVA_Top_W5_t.msb.
+have -> /=: nth false (w2bits bv) (5 - 1) = 2 ^ (5 - 1) <= to_uint bv; last by smt().
+rewrite /to_uint. 
+rewrite -{2}(cat_take_drop 4 (w2bits bv)).
+rewrite bs2int_cat size_take 1:// W5.size_w2bits /=.
+rewrite -bs2int_div 1:// /= get_to_uint /=.
+rewrite -bs2int_mod 1:// /= /to_uint.
+by smt(bs2int_range mem_range W5.size_w2bits pow2_5).
+qed.
+realize touintP by smt().
 
 (* ----------- BEGIN W8 BINDINGS ---------- *)
 bind bitstring W8.w2bits W8.bits2w W8.to_uint W8.to_sint W8.of_int W8.t 8.
@@ -98,6 +156,36 @@ rewrite [nth _ (w2bits w2) _](nth_change_dfl false) ?size_w2bits 1:/#.
 by rewrite !get_w2bits w2bitsE nth_mkseq //#.
 qed.
 
+bind op W8.t W8.orw "or".
+
+realize bvorP. 
+move => bv1 bv2. 
+apply (eq_from_nth false); 1: by smt(size_map size_zip W8.size_w2bits).
+move => i ib;rewrite !W8.get_w2bits orwE.
+rewrite (nth_map (false,false) false) /=; 1: by smt(size_map size_zip W8.size_w2bits).  
+rewrite !(nth_zip false false) //=;congr; rewrite -W8.get_w2bits.
+qed.
+
+op srl_8 (w1 w2 : W8.t) : W8.t =
+  w1 `>>>` W8.to_uint w2.
+
+bind op [W8.t] srl_8 "shr".
+realize bvshrP.
+rewrite /shr_8 => bv1 bv2.
+by rewrite W8.to_uint_shr; 1:smt(W8.to_uint_cmp).
+qed.
+
+
+op sll_8 (w1 w2 : W8.t) : W8.t =
+  w1 `<<<` to_uint w2.
+
+bind op [W8.t] sll_8 "shl".
+realize bvshlP.
+rewrite /shl_8 => bv1 bv2.
+by rewrite W8.to_uint_shl; 1:smt(W8.to_uint_cmp).
+qed.
+
+
 (* ----------- BEGIN W10 BINDINGS -----------*)
 
 theory W10.
@@ -123,6 +211,34 @@ rewrite -bs2int_div 1:// /= get_to_uint /=.
 rewrite -bs2int_mod 1:// /= /to_uint.
 have ? : 2^10 = 1024 by rewrite /=.
 by smt(bs2int_range mem_range W10.size_w2bits).
+qed.
+realize touintP by smt().
+
+(* ----------- BEGIN W10 BINDINGS -----------*)
+
+theory W11.
+abbrev [-printing] size = 11.
+clone include BitWordSH with op size <- size
+rename "_XX" as "_11"
+proof gt0_size by done,
+size_le_256 by done.
+
+end W11. export W11 W11.ALU W11.SHIFT.
+
+bind bitstring W11.w2bits W11.bits2w W11.to_uint W11.to_sint W11.of_int W11.t 11.
+realize size_tolist by auto.
+realize tolistP by auto.
+realize oflistP by smt(W11.bits2wK). 
+realize ofintP by move => *;rewrite /of_int int2bs_mod.
+realize tosintP. move => bv /=;rewrite /to_sint /smod /BVA_Top_W11_t.msb.
+have -> /=: nth false (w2bits bv) (11 - 1) = 2 ^ (11 - 1) <= to_uint bv; last by smt().
+rewrite /to_uint. 
+rewrite -{2}(cat_take_drop 10 (w2bits bv)).
+rewrite bs2int_cat size_take 1:// W11.size_w2bits /=.
+rewrite -bs2int_div 1:// /= get_to_uint /=.
+rewrite -bs2int_mod 1:// /= /to_uint.
+have ? : 2^11 = 2048 by rewrite /=.
+by smt(bs2int_range mem_range W11.size_w2bits).
 qed.
 realize touintP by smt().
 
@@ -157,6 +273,8 @@ have ?: W12.modulus = 4096 by done.
 by smt(bs2int_range mem_range W12.size_w2bits).
 qed.
 
+
+
 (* ----------- BEGIN W16 BINDINGS ---------- *)
 
 bind bitstring W16.w2bits W16.bits2w W16.to_uint W16.to_sint W16.of_int W16.t 16.
@@ -177,6 +295,10 @@ realize touintP by smt().
 
 bind op W16.t W16.( + ) "add".
 realize bvaddP by exact W16.to_uintD.
+
+bind op W16.t W16.( * ) "mul".
+realize bvmulP by exact W16.to_uintM. 
+
 
 bind op [bool & W16.t] W16.\ult "ult".
 realize bvultP by move=> bv1 bv2; rewrite W16.ultE /#.
@@ -210,26 +332,16 @@ bind op W16.t W16_sub "sub".
 realize bvsubP by  rewrite /W16_sub => bv1 bv2; rewrite W16.to_uintD to_uintN /= /#.
 
 op sll_16 (w1 w2 : W16.t) : W16.t =
-  if (16 <= to_uint w2) then  W16.zero else  w1 `<<` (truncateu8 w2).
+  w1 `<<<` to_uint w2.
 
 bind op [W16.t] sll_16 "shl".
 realize bvshlP.
-rewrite /sll_16 => bv1 bv2.
-case : (16 <= to_uint bv2); last first.
-+ rewrite /(`<<`) W16.to_uint_shl; 1: by smt(W8.to_uint_cmp).
-  rewrite /truncateu8  => bv2bnd />.
-  rewrite (pmod_small (to_uint bv2) _) //.
-  smt(W16.to_uint_cmp).
-move => *. 
-have -> : to_uint bv2 = (to_uint bv2 - 16) + 16 by ring. 
-by rewrite exprD_nneg 1,2:/# /= /#.
+rewrite /shl_16 => bv1 bv2.
+by rewrite W16.to_uint_shl; 1:smt(W16.to_uint_cmp).
 qed.
 
 op sra_16 (w1 w2 : W16.t) : W16.t =
 W16.sar w1 (to_uint w2).
-(*
-if (16 <= to_uint w2) then  W16.zero else w1 `|>>` (truncateu8 w2).
-*)
 
 bind op [W16.t] sra_16 "ashr".
 realize bvashrP.
@@ -237,22 +349,13 @@ move=> bv1 bv2; rewrite W16_sar_div; smt(W16.to_uint_cmp).
 qed.
 
 op srl_16 (w1 w2 : W16.t) : W16.t =
-  if 16 <= (to_uint w2) then W16.zero else
-  w1 `>>` (truncateu8 w2).
+  w1 `>>>` W16.to_uint w2.
 
 bind op [W16.t] srl_16 "shr".
 realize bvshrP.
-rewrite /srl_16 => bv1 bv2.
-case : (16 <= to_uint bv2); last first.
-+ rewrite /(`>>`) W16.to_uint_shr; 1: by smt(W8.to_uint_cmp).
-  rewrite /truncateu8  => bv2bnd />.
-  rewrite (pmod_small (to_uint bv2) _); smt(W16.to_uint_cmp).
-move => *. 
-have -> : to_uint bv2 = (to_uint bv2 - 16) + 16 by ring. 
-rewrite exprD_nneg 1,2:/# /=. 
-smt(StdOrder.IntOrder.expr_gt0 W16.to_uint_cmp pow2_16).
+rewrite /shr_16 => bv1 bv2.
+by rewrite W16.to_uint_shr; 1:smt(W16.to_uint_cmp).
 qed.
-
 
 bind op [W16.t & W8.t] W2u8.truncateu8 "truncate".
 realize bvtruncateP.
@@ -274,6 +377,44 @@ by have -> : (2 ^ (8 - i) * 2 ^ i) = 256;
 qed.
 
 
+bind op [W8.t & W16.t] W2u8.zeroextu16 "zextend".
+realize bvzextendP.
+move => bv; rewrite /zeroextu16 /= of_uintK /= modz_small 2://.
+apply bound_abs; smt(W8.to_uint_cmp pow2_8).
+qed.
+
+op truncateu12(a : W16.t) : W12.t =
+    W12.of_int (to_uint a).
+
+bind op [W16.t & W12.t] truncateu12 "truncate".
+realize bvtruncateP.
+move => mv; rewrite /truncateu12 /W16.w2bits take_mkseq 1:// /= /w2bits.
+apply (eq_from_nth witness);1: by smt(size_mkseq).
+move => i; rewrite size_mkseq /= /max /= => ib.
+rewrite !nth_mkseq 1..2:// /of_int /to_uint /= get_bits2w 1:// 
+        nth_mkseq 1:// /= get_to_uint 1:// /= /to_uint /=.
+have -> /=: (0 <= i && i < 16) by smt().
+pose a := bs2int (w2bits mv). 
+rewrite {1}(divz_eq a (2^(12-i)*2^i)) !mulrA divzMDl;
+   1: by smt(StdOrder.IntOrder.expr_gt0).
+rewrite dvdz_modzDl; 1: by
+ have ->  : 2^(12-i) = 2^((12-i-1)+1); [ by smt() |
+    rewrite exprS 1:/#; smt(dvdz_mull dvdz_mulr)].  
+by have -> : (2 ^ (12 - i) * 2 ^ i) = 4096; 
+  [ rewrite -StdBigop.Bigint.Num.Domain.exprD_nneg 
+     1,2:/# /= -!addrA /= | done ].
+qed.
+
+op zeroextu16(a : W12.t) : W16.t =
+    W16.of_int (to_uint a).
+
+bind op [W12.t & W16.t] zeroextu16 "zextend".
+realize bvzextendP.
+move => bv; rewrite /zeroextu16 /= of_uintK /=.
+have /= := W12.to_uint_cmp.
+by smt().
+qed.
+
 
 (* ----------- BEGIN W32 BINDINGS ---------- *)
 
@@ -292,23 +433,6 @@ rewrite -bs2int_mod 1:// /= /to_uint.
 by smt(bs2int_range mem_range W32.size_w2bits pow2_32).
 qed.
 realize touintP by smt().
-
-bind op [bool & W32.t] W32.init "init".
-realize bvinitP.
-move=> f; apply (eq_from_nth false).
- rewrite (size_flatten' 1).
-  move=> x /mkseqP [y [Hy ->]] /=.
-  exact BVA_Top_Pervasive_bool.size_tolist.
- by rewrite size_w2bits size_mkseq /#.
-rewrite size_w2bits => i Hi.
-rewrite get_w2bits (BitEncoding.BitChunking.nth_flatten false 1 _).
- apply/List.allP => x /mkseqP [y [Hy ->]] /=.
- exact BVA_Top_Pervasive_bool.size_tolist.
-by rewrite (:i %% 1 = 0) 1:/# nth_mkseq 1:/# /bool2bits initiE /=.
-qed.
-
-bind op [W32.t & bool] W32."_.[_]" "get".
-realize bvgetP by rewrite /bool2bits.
 
 bind op W32.t W32.( + ) "add".
 realize bvaddP by exact W32.to_uintD.
@@ -341,56 +465,8 @@ rewrite initiE 1:/# (nth_map (false,false)) /=;1: rewrite size_zip !size_w2bits 
 by rewrite !nth_zip /=;1:smt(W32.size_w2bits).
 qed.
 
-bind op W32.t W32.(+^) "xor".
-realize bvxorP. 
-rewrite /W32.(+^) /map2 => bv1 bv2.
-apply (eq_from_nth false);1: rewrite size_map size_zip !size_w2bits /#. 
-move => i; rewrite size_w2bits /= => ib.
-rewrite initiE 1:/# (nth_map (false,false)) /=;1: rewrite size_zip !size_w2bits /#. 
-by rewrite !nth_zip /=;1:smt(W32.size_w2bits).
-qed.
-
-bind op [W32.t] W32.invw "not".
-realize bvnotP.
-move=> bv1.
-apply (eq_from_nth false); 1: rewrite !size_map size_w2bits /#. 
-move => i; rewrite size_w2bits /= => ib.
-by rewrite (nth_map false) 1:// /= /#.
-qed.
-
-op rol_32 (w1 w2 : W32.t): W32.t =
-  w1 `|<<<|` to_uint w2. 
-
-op (`|<<|`) (w1: W32.t, w2: W8.t): W32.t =
- rol_32 w1 (zeroextu32 (w2 `&` (W8.of_int 31))).
-
-abbrev (\rol) (w1: W32.t, w2: W8.t): W32.t = w1 `|<<|`w2.
-
-bind op [W32.t] rol_32 "rol".
-realize bvrolP.
-rewrite /rol_32=> bv1 bv2 i Hi.
-by rewrite !get_w2bits rolE initiE.
-qed.
-
-op ror_32 (w1 w2 : W32.t): W32.t =
-  w1 `|>>>|` to_uint w2. 
-
-op (`|>>|`) (w1: W32.t, w2: W8.t): W32.t =
- ror_32 w1 (zeroextu32 w2).
-
-abbrev (\ror) (w1: W32.t, w2: W8.t): W32.t = w1 `|>>|`w2.
-
-bind op [W32.t] ror_32 "ror".
-realize bvrorP.
-rewrite /ror_32=> bv1 bv2 i Hi.
-by rewrite !get_w2bits rorE initiE.
-qed.
-
 op sll_32 (w1 w2 : W32.t) : W32.t =
- w1 `<<<` to_uint w2.
-
-op (`<<`) (w1: W32.t, w2: W8.t): W32.t =
- sll_32 w1 (zeroextu32 (w2 `&` (W8.of_int 31))).
+  w1 `<<<` to_uint w2.
 
 bind op [W32.t] sll_32 "shl".
 realize bvshlP.
@@ -400,9 +476,6 @@ qed.
 
 op srl_32 (w1 w2 : W32.t) : W32.t =
   w1 `>>>` W32.to_uint w2.
-
-op (`>>`) (w1: W32.t, w2: W8.t): W32.t =
- srl_32 w1 (zeroextu32 (w2 `&` (W8.of_int 31))).
 
 bind op [W32.t] srl_32 "shr".
 realize bvshrP.
@@ -419,13 +492,11 @@ move => bv1 bv2; rewrite W32_sar_div; smt(W32.to_uint_cmp).
 qed.
 
 bind op [W8.t & W32.t] W4u8.zeroextu32 "zextend".
-realize bvzextendP.
-move => bv; rewrite /zeroextu32 /= of_uintK /= modz_small 2://.
-apply bound_abs; smt(W8.to_uint_cmp pow2_8).
-qed.
+realize bvzextendP by move => bv; rewrite /zeroextu32 /= of_uintK /=; smt(W8.to_uint_cmp pow2_8).
 
 bind op [W16.t & W32.t] W2u16.zeroextu32 "zextend".
 realize bvzextendP by move => bv; rewrite /zeroextu64 /= of_uintK /=; smt(W16.to_uint_cmp pow2_16).
+
 
 bind op [W16.t & W32.t] sigextu32 "sextend".
 realize bvsextendP.
@@ -453,6 +524,7 @@ by have -> : (2 ^ (8 - i) * 2 ^ i) = 256;
      1,2:/# /= -!addrA /= | done ].
 qed.
 
+
 bind op [W32.t & W16.t] W2u16.truncateu16 "truncate".
 realize bvtruncateP.
 move => mv; rewrite /truncateu16 /W32.w2bits take_mkseq 1:// /= /w2bits.
@@ -472,23 +544,83 @@ by have -> : (2 ^ (16 - i) * 2 ^ i) = 65536;
      1,2:/# /= -!addrA /= | done ].
 qed.
 
-op BIC (x y : W32.t) : W32.t =
-  x `&` invw y.
+op truncateu32_4(a : W32.t) : W4.t =
+    W4.of_int (to_uint a).
 
-abbrev (\BIC) (x y : W32.t) : W32.t = BIC x y.
+bind op [W32.t & W4.t] truncateu32_4 "truncate".
+realize bvtruncateP.
+move => mv; rewrite /truncateu32_4 /W32.w2bits take_mkseq 1:// /= /w2bits.
+apply (eq_from_nth witness);1: by smt(size_mkseq).
+move => i; rewrite size_mkseq /= /max /= => ib.
+rewrite !nth_mkseq 1..2:// /of_int /to_uint /= get_bits2w 1:// 
+        nth_mkseq 1:// /= get_to_uint 1:// /= /to_uint /=.
+have -> /=: (0 <= i && i < 32) by smt().
+pose a := bs2int (w2bits mv). 
+rewrite {1}(divz_eq a (2^(4-i)*2^i)) !mulrA divzMDl;
+   1: by smt(StdOrder.IntOrder.expr_gt0).
+rewrite dvdz_modzDl; 1: by
+ have ->  : 2^(4-i) = 2^((4-i-1)+1); [ by smt() |
+    rewrite exprS 1:/#; smt(dvdz_mull dvdz_mulr)].  
+by have -> : (2 ^ (4 - i) * 2 ^ i) = 16; 
+  [ rewrite -StdBigop.Bigint.Num.Domain.exprD_nneg 
+     1,2:/# /= -!addrA /= | done ].
+qed.
 
-op BFC (x : W32.t) (lsb width : W8.t) : W32.t =
- let mask = ((W32.of_int (-1)) `<<` width) `|<<|` lsb
- in (x `&` mask).
+op zeroextu4_32(a : W4.t) : W32.t =
+  W32.of_int (to_uint a).
 
-abbrev (\BFC) x lsb width = BFC x lsb width.
+bind op [W4.t & W32.t] zeroextu4_32 "zextend".
+realize bvzextendP by move => bv; rewrite /zeroextu4_32 /= of_uintK /=; smt(W4.to_uint_cmp pow2_4).
 
-op BFI (x y : W32.t) (lsb width : W8.t) : W32.t =
- let mask = ((W32.of_int (-1)) `<<` width) `|<<|` lsb
- in (x `&` mask) `|` (BIC x y).
+op truncateu32_5(a : W32.t) : W5.t =
+    W5.of_int (to_uint a).
 
-abbrev (\BFI) x y lsb width = BFI x y lsb width.
+bind op [W32.t & W5.t] truncateu32_5 "truncate".
+realize bvtruncateP.
+move => mv; rewrite /truncateu32_5 /W32.w2bits take_mkseq 1:// /= /w2bits.
+apply (eq_from_nth witness);1: by smt(size_mkseq).
+move => i; rewrite size_mkseq /= /max /= => ib.
+rewrite !nth_mkseq 1..2:// /of_int /to_uint /= get_bits2w 1:// 
+        nth_mkseq 1:// /= get_to_uint 1:// /= /to_uint /=.
+have -> /=: (0 <= i && i < 32) by smt().
+pose a := bs2int (w2bits mv). 
+rewrite {1}(divz_eq a (2^(5-i)*2^i)) !mulrA divzMDl;
+   1: by smt(StdOrder.IntOrder.expr_gt0).
+rewrite dvdz_modzDl; 1: by
+ have ->  : 2^(5-i) = 2^((5-i-1)+1); [ by smt() |
+    rewrite exprS 1:/#; smt(dvdz_mull dvdz_mulr)].  
+by have -> : (2 ^ (5 - i) * 2 ^ i) = 32; 
+  [ rewrite -StdBigop.Bigint.Num.Domain.exprD_nneg 
+     1,2:/# /= -!addrA /= | done ].
+qed.
 
+op zeroextu5_32(a : W5.t) : W32.t =
+  W32.of_int (to_uint a).
+
+bind op [W5.t & W32.t] zeroextu5_32 "zextend".
+realize bvzextendP by move => bv; rewrite /zeroextu5_32 /= of_uintK /=; smt(W5.to_uint_cmp pow2_5).
+
+
+op zeroextu10_32(a : W10.t) : W32.t =
+  W32.of_int (to_uint a).
+
+bind op [W10.t & W32.t] zeroextu10_32 "zextend".
+realize bvzextendP.
+have ? : 2^10 = 1024 by auto.
+ by move => bv; rewrite /zeroextu32 /= of_uintK /=; smt(W10.to_uint_cmp).
+qed.
+
+op zeroextu11_32(a : W11.t) : W32.t =
+  W32.of_int (to_uint a).
+
+bind op [W11.t & W32.t] zeroextu11_32 "zextend".
+realize bvzextendP.
+have ? : 2^11 = 2048 by auto.
+ by move => bv; rewrite /zeroextu32 /= of_uintK /=; smt(W11.to_uint_cmp).
+qed.
+
+bind op [W32.t & bool] W32."_.[_]" "get".
+realize bvgetP by rewrite /bool2bits.
 
 (* ----------- BEGIN W64 BINDINGS ---------- *)
 
@@ -568,36 +700,21 @@ qed.
 
 
 op srl_64 (w1 w2 : W64.t) : W64.t =
-  if (64 <= to_uint w2) then  W64.zero else  w1 `>>` (truncateu8 w2).
+  w1 `>>>` to_uint w2.
 
 bind op [W64.t] srl_64 "shr".
 realize bvshrP.
-rewrite /srl_64 => bv1 bv2.
-case : (64 <= to_uint bv2); last first.
-+ rewrite /(`>>`) W64.to_uint_shr; 1: by smt(W8.to_uint_cmp).
-  rewrite /truncateu8  => bv2bnd />.
-  rewrite (pmod_small (to_uint bv2) _); smt(W64.to_uint_cmp).
-move => *. 
-have -> : to_uint bv2 = (to_uint bv2 - 64) + 64 by ring. 
-rewrite exprD_nneg 1,2:/# /=. 
-smt(StdOrder.IntOrder.expr_gt0 W64.to_uint_cmp pow2_64).
+rewrite /shr_64 => bv1 bv2.
+by rewrite W64.to_uint_shr; 1:smt(W64.to_uint_cmp).
 qed.
 
-
 op sll_64 (w1 w2 : W64.t) : W64.t =
-  if (64 <= to_uint w2) then W64.zero else w1 `<<` (truncateu8 w2).
+  w1 `<<<` to_uint w2.
 
 bind op [W64.t] sll_64 "shl".
-realize bvshlP. 
-proof.
-rewrite /sll_64 => bv1 bv2.
-case : (64 <= to_uint bv2); last first.
-+ rewrite /(`<<`) W64.to_uint_shl; 1: by smt(W8.to_uint_cmp).
-  rewrite /truncateu8  => bv2bnd />.
-  rewrite (pmod_small (to_uint bv2) _);smt(W64.to_uint_cmp).
-move => *. 
-have -> : to_uint bv2 = (to_uint bv2 - 64) + 64 by ring. 
-by rewrite exprD_nneg 1,2:/# /= /#.
+realize bvshlP.
+rewrite /shl_64 => bv1 bv2.
+by rewrite W64.to_uint_shl; 1:smt(W64.to_uint_cmp).
 qed.
 
 op rol_64 (w1 w2 : W64.t): W64.t =
@@ -609,10 +726,17 @@ rewrite /rol_64=> bv1 bv2 i Hi.
 by rewrite !get_w2bits rolE initiE.
 qed.
 
+bind op [W8.t & W64.t] W8u8.zeroextu64 "zextend".
+realize bvzextendP
+ by move => bv; rewrite /zeroextu64 /= of_uintK /=; smt(W8.to_uint_cmp pow2_8).
 
 bind op [W16.t & W64.t] W4u16.zeroextu64 "zextend".
 realize bvzextendP
  by move => bv; rewrite /zeroextu64 /= of_uintK /=; smt(W16.to_uint_cmp pow2_16).
+
+bind op [W32.t & W64.t] W2u32.zeroextu64 "zextend".
+realize bvzextendP
+ by move => bv; rewrite /zeroextu64 /= of_uintK /=; smt(W32.to_uint_cmp pow2_32).
 
 bind op [W64.t & W16.t] W4u16.truncateu16 "truncate".
 realize bvtruncateP.
@@ -633,14 +757,46 @@ by have -> : (2 ^ (16 - i) * 2 ^ i) = 65536;
      1,2:/# /= -!addrA /= | done ].
 qed.
 
-op truncate64_10 (bw: W64.t) : W10.t = W10.bits2w (W64.w2bits bw).
+op truncate64_10 (bw: W64.t) : W10.t = W10.of_int (W64.to_uint bw).
 
 bind op [W64.t & W10.t] truncate64_10 "truncate".
 realize bvtruncateP. 
-move => mv. rewrite /truncate64_10 /W64.w2bits take_mkseq 1:// /= /w2bits.
+move => mv; rewrite /truncate64_10 /W64.w2bits take_mkseq 1:// /= /w2bits.
 apply (eq_from_nth witness);1: by smt(size_mkseq).
 move => i; rewrite size_mkseq /= /max /= => ib.
-by rewrite !nth_mkseq 1..2:// /bits2w initiE 1:// /= nth_mkseq /#.  
+rewrite !nth_mkseq 1..2:// /of_int /to_uint /= get_bits2w 1:// 
+        nth_mkseq 1:// /= get_to_uint 1:// /= /to_uint /=.
+have -> /=: (0 <= i && i < 64) by smt().
+pose a := bs2int (w2bits mv). 
+rewrite {1}(divz_eq a (2^(10-i)*2^i)) !mulrA divzMDl;
+   1: by smt(StdOrder.IntOrder.expr_gt0).
+rewrite dvdz_modzDl; 1: by
+ have ->  : 2^(10-i) = 2^((10-i-1)+1); [ by smt() |
+    rewrite exprS 1:/#; smt(dvdz_mull dvdz_mulr)].  
+by have -> : (2 ^ (10 - i) * 2 ^ i) = 1024; 
+  [ rewrite -StdBigop.Bigint.Num.Domain.exprD_nneg 
+     1,2:/# /= -!addrA /= | done ].
+qed.
+
+op truncate64_11 (bw: W64.t) : W11.t = W11.of_int (W64.to_uint bw).
+
+bind op [W64.t & W11.t] truncate64_11 "truncate".
+realize bvtruncateP. 
+move => mv; rewrite /truncate64_11 /W64.w2bits take_mkseq 1:// /= /w2bits.
+apply (eq_from_nth witness);1: by smt(size_mkseq).
+move => i; rewrite size_mkseq /= /max /= => ib.
+rewrite !nth_mkseq 1..2:// /of_int /to_uint /= get_bits2w 1:// 
+        nth_mkseq 1:// /= get_to_uint 1:// /= /to_uint /=.
+have -> /=: (0 <= i && i < 64) by smt().
+pose a := bs2int (w2bits mv). 
+rewrite {1}(divz_eq a (2^(11-i)*2^i)) !mulrA divzMDl;
+   1: by smt(StdOrder.IntOrder.expr_gt0).
+rewrite dvdz_modzDl; 1: by
+ have ->  : 2^(11-i) = 2^((11-i-1)+1); [ by smt() |
+    rewrite exprS 1:/#; smt(dvdz_mull dvdz_mulr)].  
+by have -> : (2 ^ (11 - i) * 2 ^ i) = 2048; 
+  [ rewrite -StdBigop.Bigint.Num.Domain.exprD_nneg 
+     1,2:/# /= -!addrA /= | done ].
 qed.
 
 bind op [W64.t & W8.t] W8u8.truncateu8 "truncate".
@@ -681,6 +837,47 @@ rewrite -bs2int_mod 1:// /= /to_uint.
 by smt(bs2int_range mem_range W128.size_w2bits pow2_128).
 qed.
 realize touintP by smt().
+
+bind op [W64.t & W128.t] W2u64.zeroextu128 "zextend".
+realize bvzextendP by move => bv; rewrite /zeroextu128 /= of_uintK /=; smt(W64.to_uint_cmp pow2_64).
+
+bind op [W128.t & W64.t] W2u64.truncateu64 "truncate".
+realize bvtruncateP.
+move => mv; rewrite /truncateu64 /W128.w2bits take_mkseq 1:// /= /w2bits.
+apply (eq_from_nth witness);1: by smt(size_mkseq).
+move => i; rewrite size_mkseq /= /max /= => ib.
+rewrite !nth_mkseq 1..2:// /of_int /to_uint /= get_bits2w 1:// 
+        nth_mkseq 1:// /= get_to_uint 1:// /= /to_uint /=.
+have -> /=: (0 <= i && i < 128) by smt().
+pose a := bs2int (w2bits mv). 
+rewrite {1}(divz_eq a (2^(64-i)*2^i)) !mulrA divzMDl;
+   1: by smt(StdOrder.IntOrder.expr_gt0).
+rewrite dvdz_modzDl; 1: by
+ have ->  : 2^(64-i) = 2^((64-i-1)+1); [ by smt() |
+    rewrite exprS 1:/#; smt(dvdz_mull dvdz_mulr)].  
+by have -> : (2 ^ (64 - i) * 2 ^ i) = 18446744073709551616; 
+  [ rewrite -StdBigop.Bigint.Num.Domain.exprD_nneg 
+     1,2:/# /= -!addrA /= | done ].
+qed.
+
+bind op [W128.t & W32.t] W4u32.truncateu32 "truncate".
+realize bvtruncateP.
+move => mv; rewrite /truncateu32 /W128.w2bits take_mkseq 1:// /= /w2bits.
+apply (eq_from_nth witness);1: by smt(size_mkseq).
+move => i; rewrite size_mkseq /= /max /= => ib.
+rewrite !nth_mkseq 1..2:// /of_int /to_uint /= get_bits2w 1:// 
+        nth_mkseq 1:// /= get_to_uint 1:// /= /to_uint /=.
+have -> /=: (0 <= i && i < 128) by smt().
+pose a := bs2int (w2bits mv). 
+rewrite {1}(divz_eq a (2^(32-i)*2^i)) !mulrA divzMDl;
+   1: by smt(StdOrder.IntOrder.expr_gt0).
+rewrite dvdz_modzDl; 1: by
+ have ->  : 2^(32-i) = 2^((32-i-1)+1); [ by smt() |
+    rewrite exprS 1:/#; smt(dvdz_mull dvdz_mulr)].  
+by have -> : (2 ^ (32 - i) * 2 ^ i) = 4294967296; 
+  [ rewrite -StdBigop.Bigint.Num.Domain.exprD_nneg 
+     1,2:/# /= -!addrA /= | done ].
+qed.
 
 (* ----------- BEGIN W256 BINDINGS ---------- *)
 
@@ -753,7 +950,7 @@ by rewrite (nth_map false) 1:// /= /#.
 qed.
 
 
-bind op [W256.t & W128.t] truncateu128 "truncate".
+bind op [W256.t & W128.t] W2u128.truncateu128 "truncate".
 realize bvtruncateP.
 move => mv; rewrite /truncateu128 /W256.w2bits take_mkseq 1:// /= /w2bits.
 apply (eq_from_nth witness);1: by smt(size_mkseq).
@@ -772,37 +969,6 @@ by have -> : (2 ^ (128 - i) * 2 ^ i) = 340282366920938463463374607431768211456;
      1,2:/# /= -!addrA /= | done ].
 qed.
 
-(*
-(* ----------- BEGIN W512 BINDINGS ---------- *)
-
-theory W512.
-  abbrev [-printing] size = 512.
-  clone include BitWord with op size <- size
-  rename "_XX" as "_256"
-  proof gt0_size by done.
-end W512.
-
-import W512.
-
-bind bitstring W512.w2bits W512.bits2w W512.to_uint W512.to_sint W512.of_int W512.t 512.
-realize size_tolist by auto.
-realize tolistP     by auto.
-realize oflistP     by smt(W512.bits2wK).
-realize ofintP      by move=> *; rewrite /of_int int2bs_mod.
-realize touintP     by smt().
-
-realize tosintP.
-proof.
-move=> bv /= @/to_sint @/smod @/msb.
-rewrite (_ : nth _ _ _ = 2 ^ (512 - 1) <= to_uint bv) -1:/#.
-rewrite /to_uint -{2}(cat_take_drop 511 (w2bits bv)).
-rewrite bs2int_cat size_take ~-1:// W512.size_w2bits /=.
-rewrite -bs2int_div ~-1:// /= get_to_uint ~-1:// /=.
-rewrite -bs2int_mod ~-1:// /= /to_uint.
-have ?: W512.modulus = 13407807929942597099574024998205846127479365820592393377723561443721764030073546976801874298166903427690031858186486050853753882811946569946433649006084096 by done.
-by smt(bs2int_range mem_range W512.size_w2bits).
-qed.
-*)
 
 (* ----------- BEGIN ARRAY BINDINGS ---------- *)
 
@@ -812,6 +978,12 @@ realize get_setP by smt(Array256.get_setE).
 realize eqP by smt(Array256.tP).
 realize get_out by smt(Array256.get_out).
 
+bind array Array384."_.[_]" Array384."_.[_<-_]" Array384.to_list Array384.of_list Array384.t 384.
+realize tolistP by done.
+realize get_setP by smt(Array384.get_setE). 
+realize eqP by smt(Array384.tP).
+realize get_out by smt(Array384.get_out).
+
 
 bind array Array768."_.[_]" Array768."_.[_<-_]" Array768.to_list Array768.of_list Array768.t 768.
 realize tolistP by done.
@@ -819,11 +991,71 @@ realize get_setP by smt(Array768.get_setE).
 realize eqP by smt(Array768.tP).
 realize get_out by smt(Array768.get_out).
 
+bind array Array1024."_.[_]" Array1024."_.[_<-_]" Array1024.to_list Array1024.of_list Array1024.t 1024.
+realize tolistP by done.
+realize get_setP by smt(Array1024.get_setE). 
+realize eqP by smt(Array1024.tP).
+realize get_out by smt(Array1024.get_out).
+
+bind array Array1088."_.[_]" Array1088."_.[_<-_]" Array1088.to_list Array1088.of_list Array1088.t 1088.
+realize tolistP by done.
+realize get_setP by smt(Array1088.get_setE). 
+realize eqP by smt(Array1088.tP).
+realize get_out by smt(Array1088.get_out).
+
+bind array Array1152."_.[_]" Array1152."_.[_<-_]" Array1152.to_list Array1152.of_list Array1152.t 1152.
+realize tolistP by done.
+realize get_setP by smt(Array1152.get_setE). 
+realize eqP by smt(Array1152.tP).
+realize get_out by smt(Array1152.get_out).
+
+bind array Array1408."_.[_]" Array1408."_.[_<-_]" Array1408.to_list Array1408.of_list Array1408.t 1408.
+realize tolistP by done.
+realize get_setP by smt(Array1408.get_setE). 
+realize eqP by smt(Array1408.tP).
+realize get_out by smt(Array1408.get_out).
+
+bind array Array1536."_.[_]" Array1536."_.[_<-_]" Array1536.to_list Array1536.of_list Array1536.t 1536.
+realize tolistP by done.
+realize get_setP by smt(Array1536.get_setE). 
+realize eqP by smt(Array1536.tP).
+realize get_out by smt(Array1536.get_out).
+
+bind array Array1568."_.[_]" Array1568."_.[_<-_]" Array1568.to_list Array1568.of_list Array1568.t 1568.
+realize tolistP by done.
+realize get_setP by smt(Array1568.get_setE). 
+realize eqP by smt(Array1568.tP).
+realize get_out by smt(Array1568.get_out).
+
 bind array Array32."_.[_]" Array32."_.[_<-_]" Array32.to_list Array32.of_list Array32.t 32.
 realize tolistP by done.
 realize get_setP by smt(Array32.get_setE). 
 realize eqP by smt(Array32.tP).
 realize get_out by smt(Array32.get_out).
+
+bind array Array16."_.[_]" Array16."_.[_<-_]" Array16.to_list Array16.of_list Array16.t 16.
+realize tolistP by done.
+realize get_setP by smt(Array16.get_setE). 
+realize eqP by smt(Array16.tP).
+realize get_out by smt(Array16.get_out).
+
+bind array Array48."_.[_]" Array48."_.[_<-_]" Array48.to_list Array48.of_list Array48.t 48.
+realize tolistP by done.
+realize get_setP by smt(Array48.get_setE). 
+realize eqP by smt(Array48.tP).
+realize get_out by smt(Array48.get_out).
+
+bind array Array128."_.[_]" Array128."_.[_<-_]" Array128.to_list Array128.of_list Array128.t 128.
+realize tolistP by done.
+realize get_setP by smt(Array128.get_setE). 
+realize eqP by smt(Array128.tP).
+realize get_out by smt(Array128.get_out).
+
+bind array Array160."_.[_]" Array160."_.[_<-_]" Array160.to_list Array160.of_list Array160.t 160.
+realize tolistP by done.
+realize get_setP by smt(Array160.get_setE). 
+realize eqP by smt(Array160.tP).
+realize get_out by smt(Array160.get_out).
 
 bind array Array960."_.[_]" Array960."_.[_<-_]" Array960.to_list Array960.of_list Array960.t 960.
 realize tolistP by done.
@@ -831,11 +1063,30 @@ realize get_setP by smt(Array960.get_setE).
 realize eqP by smt(Array960.tP).
 realize get_out by smt(Array960.get_out).
 
+bind array Array1410."_.[_]" Array1410."_.[_<-_]" Array1410.to_list Array1410.of_list Array1410.t 1410.
+realize tolistP by done.
+realize get_setP by smt(Array1410.get_setE). 
+realize eqP by smt(Array1410.tP).
+realize get_out by smt(Array1410.get_out).
+
 bind array Array4."_.[_]" Array4."_.[_<-_]" Array4.to_list Array4.of_list Array4.t 4.
 realize tolistP by done.
 realize get_setP by smt(Array4.get_setE). 
 realize eqP by smt(Array4.tP).
 realize get_out by smt(Array4.get_out).
+
+bind array Array1."_.[_]" Array1."_.[_<-_]" Array1.to_list Array1.of_list Array1.t 1.
+realize tolistP by done.
+realize get_setP by smt(Array1.get_setE). 
+realize eqP by smt(Array1.tP).
+realize get_out by smt(Array1.get_out).
+
+bind array Array2."_.[_]" Array2."_.[_<-_]" Array2.to_list Array2.of_list Array2.t 2.
+realize tolistP by done.
+realize get_setP by smt(Array2.get_setE). 
+realize eqP by smt(Array2.tP).
+realize get_out by smt(Array2.get_out).
+
 
 bind array Array5."_.[_]" Array5."_.[_<-_]" Array5.to_list Array5.of_list Array5.t 5.
 realize tolistP by done.
@@ -855,6 +1106,12 @@ realize get_setP by smt(Array7.get_setE).
 realize eqP by smt(Array7.tP).
 realize get_out by smt(Array7.get_out).
 
+bind array Array8."_.[_]" Array8."_.[_<-_]" Array8.to_list Array8.of_list Array8.t 8.
+realize tolistP by done.
+realize get_setP by smt(Array8.get_setE). 
+realize eqP by smt(Array8.tP).
+realize get_out by smt(Array8.get_out).
+
 bind array Array24."_.[_]" Array24."_.[_<-_]" Array24.to_list Array24.of_list Array24.t 24.
 realize tolistP by done.
 realize get_setP by smt(Array24.get_setE). 
@@ -867,55 +1124,115 @@ realize get_setP by smt(Array25.get_setE).
 realize eqP by smt(Array25.tP).
 realize get_out by smt(Array25.get_out).
 
-bind array Array8."_.[_]" Array8."_.[_<-_]" Array8.to_list Array8.of_list Array8.t 8.
-realize tolistP by done.
-realize get_setP by smt(Array8.get_setE). 
-realize eqP by smt(Array8.tP).
-realize get_out by smt(Array8.get_out).
+op init_32_8 (f: int -> W8.t) : W8.t Array32.t = Array32.init f.
 
-bind array Array50."_.[_]" Array50."_.[_<-_]" Array50.to_list Array50.of_list Array50.t 50.
-realize tolistP by done.
-realize get_setP by smt(Array50.get_setE). 
-realize eqP by smt(Array50.tP).
-realize get_out by smt(Array50.get_out).
-
-bind array Array48."_.[_]" Array48."_.[_<-_]" Array48.to_list Array48.of_list Array48.t 48.
-realize tolistP by done.
-realize get_setP by smt(Array48.get_setE). 
-realize eqP by smt(Array48.tP).
-realize get_out by smt(Array48.get_out).
-
-op init_8_32 f: W32.t Array8.t = Array8.init f.
-bind op [W32.t & Array8.t] init_8_32 "ainit".
+bind op [W8.t & Array32.t] init_32_8 "ainit".
 realize bvainitP.
 proof.
-rewrite /init_8_32 => f.
+rewrite /init_32_8 => f.
+rewrite BVA_Top_Array32_Array32_t.tolistP.
+apply eq_in_mkseq => i i_bnd;
+smt(Array32.initE).
+qed.
+
+op init_1568_8 (f: int -> W8.t) : W8.t Array1568.t = Array1568.init f.
+
+bind op [W8.t & Array1568.t] init_1568_8 "ainit".
+realize bvainitP.
+proof.
+rewrite /init_1568_8 => f.
+rewrite BVA_Top_Array1568_Array1568_t.tolistP.
+apply eq_in_mkseq => i i_bnd;
+smt(Array1568.initE).
+qed.
+
+op init_1536_8 (f: int -> W8.t) : W8.t Array1536.t = Array1536.init f.
+
+bind op [W8.t & Array1536.t] init_1536_8 "ainit".
+realize bvainitP.
+proof.
+rewrite /init_1536_8 => f.
+rewrite BVA_Top_Array1536_Array1536_t.tolistP.
+apply eq_in_mkseq => i i_bnd;
+smt(Array1536.initE).
+qed.
+
+op init_1024_8 (f: int -> W8.t) : W8.t Array1024.t = Array1024.init f.
+
+bind op [W8.t & Array1024.t] init_1024_8 "ainit".
+realize bvainitP.
+proof.
+rewrite /init_1024_8 => f.
+rewrite BVA_Top_Array1024_Array1024_t.tolistP.
+apply eq_in_mkseq => i i_bnd;
+smt(Array1024.initE).
+qed.
+
+op init_8_8 (f: int -> W8.t) : W8.t Array8.t = Array8.init f.
+
+bind op [W8.t & Array8.t] init_8_8 "ainit".
+realize bvainitP.
+proof.
+rewrite /init_8_8 => f.
 rewrite BVA_Top_Array8_Array8_t.tolistP.
 apply eq_in_mkseq => i i_bnd;
 smt(Array8.initE).
 qed.
 
-op init_50_32 f: W32.t Array50.t = Array50.init f.
-bind op [W32.t & Array50.t] init_50_32 "ainit".
+op init_8_16 (f: int -> W16.t) : W16.t Array8.t = Array8.init f.
+
+bind op [W16.t & Array8.t] init_8_16 "ainit".
 realize bvainitP.
 proof.
-rewrite /init_50_32 => f.
-rewrite BVA_Top_Array50_Array50_t.tolistP.
+rewrite /init_8_16 => f.
+rewrite BVA_Top_Array8_Array8_t.tolistP.
 apply eq_in_mkseq => i i_bnd;
-smt(Array50.initE).
+smt(Array8.initE).
 qed.
 
-op init_48_32 f: W32.t Array48.t = Array48.init f.
-bind op [W32.t & Array48.t] init_48_32 "ainit".
+op init_160_8 (f: int -> W8.t) : W8.t Array160.t = Array160.init f.
+
+bind op [W8.t & Array160.t] init_160_8 "ainit".
 realize bvainitP.
 proof.
-rewrite /init_48_32 => f.
-rewrite BVA_Top_Array48_Array48_t.tolistP.
+rewrite /init_160_8 => f.
+rewrite BVA_Top_Array160_Array160_t.tolistP.
 apply eq_in_mkseq => i i_bnd;
-smt(Array48.initE).
+smt(Array160.initE).
 qed.
 
+op init_1152_8 (f: int -> W8.t) : W8.t Array1152.t = Array1152.init f.
 
+bind op [W8.t & Array1152.t] init_1152_8 "ainit".
+realize bvainitP.
+proof.
+rewrite /init_1152_8 => f.
+rewrite BVA_Top_Array1152_Array1152_t.tolistP.
+apply eq_in_mkseq => i i_bnd;
+smt(Array1152.initE).
+qed.
+
+op init_128_8 (f: int -> W8.t) : W8.t Array128.t = Array128.init f.
+
+bind op [W8.t & Array128.t] init_128_8 "ainit".
+realize bvainitP.
+proof.
+rewrite /init_128_8 => f.
+rewrite BVA_Top_Array128_Array128_t.tolistP.
+apply eq_in_mkseq => i i_bnd;
+smt(Array128.initE).
+qed.
+
+op init_384_8 (f: int -> W8.t) : W8.t Array384.t = Array384.init f.
+
+bind op [W8.t & Array384.t] init_384_8 "ainit".
+realize bvainitP.
+proof.
+rewrite /init_384_8 => f.
+rewrite BVA_Top_Array384_Array384_t.tolistP.
+apply eq_in_mkseq => i i_bnd;
+smt(Array384.initE).
+qed.
 
 op init_256_16 (f: int -> W16.t) : W16.t Array256.t = Array256.init f.
 
@@ -937,6 +1254,15 @@ rewrite BVA_Top_Array768_Array768_t.tolistP.
 apply eq_in_mkseq => i i_bnd; smt(Array768.initE).
 qed.
 
+op init_1024_16 (f: int -> W16.t) : W16.t Array1024.t = Array1024.init f.
+
+bind op [W16.t & Array1024.t] init_1024_16 "ainit".
+realize bvainitP.
+rewrite /init_1024_16 => f.
+rewrite BVA_Top_Array1024_Array1024_t.tolistP.
+apply eq_in_mkseq => i i_bnd; smt(Array1024.initE).
+qed.
+
 op init_4_64 (f: int -> W64.t) : W64.t Array4.t = Array4.init f.
 
 bind op [W64.t & Array4.t] init_4_64 "ainit".
@@ -945,6 +1271,16 @@ proof.
 rewrite /init_4_64 => f.
 rewrite BVA_Top_Array4_Array4_t.tolistP.
 apply eq_in_mkseq => i i_bnd; smt(Array4.initE).
+qed.
+
+op init_5_32 (f: int -> W32.t) : W32.t Array5.t = Array5.init f.
+
+bind op [W32.t & Array5.t] init_5_32 "ainit".
+realize bvainitP.
+proof.
+rewrite /init_5_32 => f.
+rewrite BVA_Top_Array5_Array5_t.tolistP.
+apply eq_in_mkseq => i i_bnd; smt(Array5.initE).
 qed.
 
 op init_5_64 (f: int -> W64.t) = Array5.init f.
@@ -957,17 +1293,6 @@ rewrite BVA_Top_Array5_Array5_t.tolistP.
 apply eq_in_mkseq => i i_bnd;
 smt(Array5.initE).
 qed.
-
-op init_5_32 f: W32.t Array5.t = Array5.init f.
-bind op [W32.t & Array5.t] init_5_32 "ainit".
-realize bvainitP.
-proof.
-rewrite /init_5_32 => f.
-rewrite BVA_Top_Array5_Array5_t.tolistP.
-apply eq_in_mkseq => i i_bnd;
-smt(Array5.initE).
-qed.
-
 
 op init_6_256 (f: int -> W256.t) = Array6.init f.
 
@@ -1001,16 +1326,6 @@ rewrite BVA_Top_Array25_Array25_t.tolistP.
 by apply eq_in_mkseq => i i_bnd; smt(Array25.initE).
 qed.
 
-op init_25_256 (f: int -> W256.t) = Array25.init f.
-
-bind op [W256.t & Array25.t] init_25_256 "ainit".
-realize bvainitP.
-proof.
-rewrite /init_25_256 => f.
-rewrite BVA_Top_Array25_Array25_t.tolistP.
-by apply eq_in_mkseq => i i_bnd; smt(Array25.initE).
-qed.
-
 op init_960_8 (f: int -> W8.t) : W8.t Array960.t = Array960.init f.
 
 bind op [W8.t & Array960.t] init_960_8 "ainit".
@@ -1020,6 +1335,222 @@ rewrite /init_960_8 => f.
 rewrite BVA_Top_Array960_Array960_t.tolistP.
 apply eq_in_mkseq => i i_bnd; smt(Array960.initE).
 qed.
+
+op init_1408_8 (f: int -> W8.t) : W8.t Array1408.t = Array1408.init f.
+
+bind op [W8.t & Array1408.t] init_1408_8 "ainit".
+realize bvainitP.
+proof.
+rewrite /init_1408_8 => f.
+rewrite BVA_Top_Array1408_Array1408_t.tolistP.
+apply eq_in_mkseq => i i_bnd; smt(Array1408.initE).
+qed.
+
+op sliceget8_32_256 (arr: W32.t Array8.t) (offset: int) : W256.t = 
+   if 8 %| offset then 
+    get256_direct ((init32 (fun (i_0 : int) => arr.[i_0])))%WArray32 (offset %/ 8)
+   else W256.bits2w (take 256 (drop offset (flatten (map W32.w2bits (to_list arr))))).
+
+bind op [W32.t & W256.t & Array8.t] sliceget8_32_256 "asliceget".
+realize bvaslicegetP.
+move => /= arr offset; rewrite /sliceget8_32_256 /= => H k kb. 
+case (8%| offset) => /= *; last by smt(W256.get_bits2w).
+rewrite /get256_direct pack32E initiE 1:/# /= initiE 1:/# /= initiE 1:/# /=.
+rewrite nth_take 1,2:/# nth_drop 1,2:/#.
+rewrite (BitEncoding.BitChunking.nth_flatten false 32 _). 
++ rewrite allP => x /=; rewrite mapP => He; elim He;smt(W32.size_w2bits).
+rewrite (nth_map W32.zero []); 1: smt(Array8.size_to_list).
+rewrite nth_mkseq 1:/# /(\bits8) initiE 1:/# /= /#.
+qed.
+
+op sliceget4_64_256 (arr: W64.t Array4.t) (offset: int) : W256.t = 
+   if 8 %| offset then 
+    get256_direct ((init64 (fun (i_0 : int) => arr.[i_0])))%WArray32 (offset %/ 8)
+   else W256.bits2w (take 256 (drop offset (flatten (map W64.w2bits (to_list arr))))).
+
+bind op [W64.t & W256.t & Array4.t] sliceget4_64_256 "asliceget".
+realize bvaslicegetP.
+move => /= arr offset; rewrite /sliceget4_64_256 /= => H k kb. 
+case (8%| offset) => /= *; last by smt(W256.get_bits2w).
+rewrite /get256_direct pack32E initiE 1:/# /= initiE 1:/# /= initiE 1:/# /=.
+rewrite nth_take 1,2:/# nth_drop 1,2:/#.
+rewrite (BitEncoding.BitChunking.nth_flatten false 64 _). 
++ rewrite allP => x /=; rewrite mapP => He; elim He;smt(W64.size_w2bits).
+rewrite (nth_map W64.zero []); 1: smt(Array4.size_to_list).
+rewrite nth_mkseq 1:/# /(\bits8) initiE 1:/# /= /#.
+qed.
+
+op sliceget4_32_128 (arr: W32.t Array4.t) (offset: int) : W128.t = 
+   if 8 %| offset then 
+    get128_direct ((init32 (fun (i_0 : int) => arr.[i_0])))%WArray16 (offset %/ 8)
+   else W128.bits2w (take 128 (drop offset (flatten (map W32.w2bits (to_list arr))))).
+
+bind op [W32.t & W128.t & Array4.t] sliceget4_32_128 "asliceget".
+realize bvaslicegetP.
+move => /= arr offset; rewrite /sliceget4_32_128 /= => H k kb. 
+case (8%| offset) => /= *; last by smt(W128.get_bits2w).
+rewrite /get128_direct pack16E initiE 1:/# /= initiE 1:/# /= initiE 1:/# /=.
+rewrite nth_take 1,2:/# nth_drop 1,2:/#.
+rewrite (BitEncoding.BitChunking.nth_flatten false 32 _). 
++ rewrite allP => x /=; rewrite mapP => He; elim He;smt(W32.size_w2bits).
+rewrite (nth_map W32.zero []); 1: smt(Array4.size_to_list).
+rewrite nth_mkseq 1:/# /(\bits8) initiE 1:/# /= /#.
+qed.
+
+op sliceget16_8_128 (arr: W8.t Array16.t) (offset: int) : W128.t = 
+   if 8 %| offset then 
+    get128_direct ((init8 (fun (i_0 : int) => arr.[i_0])))%WArray16 (offset %/ 8)
+   else W128.bits2w (take 128 (drop offset (flatten (map W8.w2bits (to_list arr))))).
+
+bind op [W8.t & W128.t & Array16.t] sliceget16_8_128 "asliceget".
+realize bvaslicegetP.
+move => /= arr offset; rewrite /sliceget16_8_128 /= => H k kb. 
+case (8%| offset) => /= *; last by smt(W128.get_bits2w).
+rewrite /get128_direct pack16E initiE 1:/# /= initiE 1:/# /= initiE 1:/# /=.
+rewrite nth_take 1,2:/# nth_drop 1,2:/#.
+rewrite (BitEncoding.BitChunking.nth_flatten false 8 _). 
++ rewrite allP => x /=; rewrite mapP => He; elim He;smt(W8.size_w2bits).
+rewrite (nth_map W8.zero []); 1: smt(Array16.size_to_list).
+rewrite nth_mkseq 1:/# /= /#.
+qed.
+
+op sliceget16_16_256 (arr: W16.t Array16.t) (offset: int) : W256.t = 
+   if 8 %| offset then 
+    get256_direct ((init16 (fun (i_0 : int) => arr.[i_0])))%WArray32 (offset %/ 8)
+   else W256.bits2w (take 256 (drop offset (flatten (map W16.w2bits (to_list arr))))).
+
+bind op [W16.t & W256.t & Array16.t] sliceget16_16_256 "asliceget".
+realize bvaslicegetP.
+move => /= arr offset; rewrite /sliceget16_16_256 /= => H k kb. 
+case (8%| offset) => /= *; last by smt(W256.get_bits2w).
+rewrite /get256_direct pack32E initiE 1:/# /= initiE 1:/# /= initiE 1:/# /=.
+rewrite nth_take 1,2:/# nth_drop 1,2:/#.
+rewrite (BitEncoding.BitChunking.nth_flatten false 16 _). 
++ rewrite allP => x /=; rewrite mapP => He; elim He;smt(W16.size_w2bits).
+rewrite (nth_map W16.zero []); 1: smt(Array16.size_to_list).
+rewrite nth_mkseq 1:/# /(\bits8) initiE 1:/# /= /#.
+qed.
+
+op sliceget1024_16_256 (arr: W16.t Array1024.t) (offset: int) : W256.t = 
+   if 8 %| offset then 
+    get256_direct ((init16 (fun (i_0 : int) => arr.[i_0])))%WArray2048 (offset %/ 8)
+   else W256.bits2w (take 256 (drop offset (flatten (map W16.w2bits (to_list arr))))).
+
+bind op [W16.t & W256.t & Array1024.t] sliceget1024_16_256 "asliceget".
+realize bvaslicegetP.
+move => /= arr offset; rewrite /sliceget1024_16_256 /= => H k kb. 
+case (8%| offset) => /= *; last by smt(W256.get_bits2w).
+rewrite /get256_direct pack32E initiE 1:/# /= initiE 1:/# /= initiE 1:/# /=.
+rewrite nth_take 1,2:/# nth_drop 1,2:/#.
+rewrite (BitEncoding.BitChunking.nth_flatten false 16 _). 
++ rewrite allP => x /=; rewrite mapP => He; elim He;smt(W16.size_w2bits).
+rewrite (nth_map W16.zero []); 1: smt(Array1024.size_to_list).
+rewrite nth_mkseq 1:/# /(\bits8) initiE 1:/# /= /#.
+qed.
+
+op sliceget160_8_64 (arr: W8.t Array160.t) (offset: int) : W64.t = 
+   if 8 %| offset then 
+    get64_direct ((init8 (fun (i_0 : int) => arr.[i_0])))%WArray160 (offset %/ 8)
+   else W64.bits2w (take 64 (drop offset (flatten (map W8.w2bits (to_list arr))))).
+
+bind op [W8.t & W64.t & Array160.t] sliceget160_8_64 "asliceget".
+realize bvaslicegetP.
+move => /= arr offset; rewrite /sliceget160_8_64 /= => H k kb. 
+case (8%| offset) => /= *; last by smt(W64.get_bits2w).
+rewrite /get64_direct pack8E initiE 1:/# /= initiE 1:/# /= initiE 1:/# /=.
+rewrite nth_take 1,2:/# nth_drop 1,2:/#.
+rewrite (BitEncoding.BitChunking.nth_flatten false 8 _). 
++ rewrite allP => x /=; rewrite mapP => He; elim He;smt(W8.size_w2bits).
+rewrite (nth_map W8.zero []); 1: smt(Array160.size_to_list).
+rewrite nth_mkseq /#.
+qed.
+
+op sliceget128_8_64 (arr: W8.t Array128.t) (offset: int) : W64.t = 
+   if 8 %| offset then 
+    get64_direct ((init8 (fun (i_0 : int) => arr.[i_0])))%WArray128 (offset %/ 8)
+   else W64.bits2w (take 64 (drop offset (flatten (map W8.w2bits (to_list arr))))).
+
+bind op [W8.t & W64.t & Array128.t] sliceget128_8_64 "asliceget".
+realize bvaslicegetP.
+move => /= arr offset; rewrite /sliceget128_8_64 /= => H k kb. 
+case (8%| offset) => /= *; last by smt(W64.get_bits2w).
+rewrite /get64_direct pack8E initiE 1:/# /= initiE 1:/# /= initiE 1:/# /=.
+rewrite nth_take 1,2:/# nth_drop 1,2:/#.
+rewrite (BitEncoding.BitChunking.nth_flatten false 8 _). 
++ rewrite allP => x /=; rewrite mapP => He; elim He;smt(W8.size_w2bits).
+rewrite (nth_map W8.zero []); 1: smt(Array128.size_to_list).
+rewrite nth_mkseq /#.
+qed.
+
+
+op sliceget160_8_16 (arr: W8.t Array160.t) (offset: int) : W16.t = 
+   if 8 %| offset then 
+    get16_direct ((init8 (fun (i_0 : int) => arr.[i_0])))%WArray160 (offset %/ 8)
+   else W16.bits2w (take 16 (drop offset (flatten (map W8.w2bits (to_list arr))))).
+
+bind op [W8.t & W16.t & Array160.t] sliceget160_8_16 "asliceget".
+realize bvaslicegetP.
+move => /= arr offset; rewrite /sliceget160_8_16 /= => H k kb. 
+case (8%| offset) => /= *; last by smt(W16.get_bits2w).
+rewrite /get16_direct pack2E initiE 1:/# /= initiE 1:/# /= initiE 1:/# /=.
+rewrite nth_take 1,2:/# nth_drop 1,2:/#.
+rewrite (BitEncoding.BitChunking.nth_flatten false 8 _). 
++ rewrite allP => x /=; rewrite mapP => He; elim He;smt(W8.size_w2bits).
+rewrite (nth_map W8.zero []); 1: smt(Array160.size_to_list).
+rewrite nth_mkseq /#.
+qed.
+
+op sliceget128_8_16 (arr: W8.t Array128.t) (offset: int) : W16.t = 
+   if 8 %| offset then 
+    get16_direct ((init8 (fun (i_0 : int) => arr.[i_0])))%WArray128 (offset %/ 8)
+   else W16.bits2w (take 16 (drop offset (flatten (map W8.w2bits (to_list arr))))).
+
+bind op [W8.t & W16.t & Array128.t] sliceget128_8_16 "asliceget".
+realize bvaslicegetP.
+move => /= arr offset; rewrite /sliceget128_8_16 /= => H k kb. 
+case (8%| offset) => /= *; last by smt(W16.get_bits2w).
+rewrite /get16_direct pack2E initiE 1:/# /= initiE 1:/# /= initiE 1:/# /=.
+rewrite nth_take 1,2:/# nth_drop 1,2:/#.
+rewrite (BitEncoding.BitChunking.nth_flatten false 8 _). 
++ rewrite allP => x /=; rewrite mapP => He; elim He;smt(W8.size_w2bits).
+rewrite (nth_map W8.zero []); 1: smt(Array128.size_to_list).
+rewrite nth_mkseq /#.
+qed.
+
+op sliceget1568_8_256 (arr: W8.t Array1568.t) (offset: int) : W256.t = 
+   if 8 %| offset then 
+    get256_direct ((WArray1568.init8 (fun (i_0 : int) => arr.[i_0])))%WArray32 (offset %/ 8)
+   else W256.bits2w (take 256 (drop offset (flatten (map W8.w2bits (to_list arr))))).
+
+bind op [W8.t & W256.t & Array1568.t] sliceget1568_8_256 "asliceget".
+realize bvaslicegetP.
+move => /= arr offset; rewrite /sliceget1568_8_256 /= => H k kb. 
+case (8%| offset) => /= *; last by smt(W256.get_bits2w).
+rewrite /get256_direct pack32E initiE 1:/# /= initiE 1:/# /= initiE 1:/# /=.
+rewrite nth_take 1,2:/# nth_drop 1,2:/#.
+rewrite (BitEncoding.BitChunking.nth_flatten false 8 _). 
++ rewrite allP => x /=; rewrite mapP => He; elim He;smt(W8.size_w2bits).
+rewrite (nth_map W8.zero []); 1: smt(Array1568.size_to_list).
+rewrite nth_mkseq /#.
+qed.
+
+op sliceget1088_8_256 (arr: W8.t Array1088.t) (offset: int) : W256.t = 
+   if 8 %| offset then 
+    get256_direct ((WArray1088.init8 (fun (i_0 : int) => arr.[i_0])))%WArray32 (offset %/ 8)
+   else W256.bits2w (take 256 (drop offset (flatten (map W8.w2bits (to_list arr))))).
+
+bind op [W8.t & W256.t & Array1088.t] sliceget1088_8_256 "asliceget".
+realize bvaslicegetP.
+move => /= arr offset; rewrite /sliceget1088_8_256 /= => H k kb. 
+case (8%| offset) => /= *; last by smt(W256.get_bits2w).
+rewrite /get256_direct pack32E initiE 1:/# /= initiE 1:/# /= initiE 1:/# /=.
+rewrite nth_take 1,2:/# nth_drop 1,2:/#.
+rewrite (BitEncoding.BitChunking.nth_flatten false 8 _). 
++ rewrite allP => x /=; rewrite mapP => He; elim He;smt(W8.size_w2bits).
+rewrite (nth_map W8.zero []); 1: smt(Array1088.size_to_list).
+rewrite nth_mkseq /#.
+qed.
+
 
 op sliceget256_16_256 (arr: W16.t Array256.t) (offset: int) : W256.t = 
    if 8 %| offset then 
@@ -1097,6 +1628,133 @@ rewrite (nth_map W8.zero []); 1: smt(Array32.size_to_list).
 by rewrite nth_mkseq /#.
 qed.
 
+op sliceset32_8_32 (arr: W8.t Array32.t) (offset: int) (bv: W32.t) : W8.t Array32.t =
+  if 8 %| offset
+  then (init (fun (i3 : int) => get8 (set32_direct ((init8 (fun (i_0 : int) => arr.[i_0])))%WArray32 (offset %/ 8) bv) i3))%Array32
+  else  Array32.of_list witness (map W8.bits2w (chunk 8 (take offset (flatten (map W8.w2bits (to_list arr))) ++ w2bits bv ++
+  drop (offset + 32) (flatten (map W8.w2bits (to_list arr)))))).
+
+lemma size_flatten_W8_w2bits (a : W8.t list) :
+  (size (flatten (map W8.w2bits (a))))  =  8 * size a.
+proof.
+  rewrite size_flatten -map_comp /(\o) /=.
+  rewrite StdBigop.Bigint.sumzE /= StdBigop.Bigint.BIA.big_mapT /(\o) /=. 
+  rewrite StdBigop.Bigint.big_constz count_predT /#.
+qed.
+
+bind op [W8.t & W32.t & Array32.t] sliceset32_8_32 "asliceset".
+realize bvaslicesetP. 
+move => arr offset bv H /= k kb; rewrite /sliceset32_8_32 /=. 
+case (8 %| offset) => /= *; last first.
++ rewrite of_listK; 1: by rewrite size_map size_chunk 1:// !size_cat size_take;
+      by smt(size_take size_drop  W8.size_w2bits size_cat Array32.size_to_list size_flatten_W8_w2bits size_ge0). 
+  rewrite -(map_comp W8.w2bits W8.bits2w) /(\o). 
+  have := eq_in_map ((fun (x : bool list) => w2bits ((bits2w x))%W8)) idfun (chunk 8
+        (take offset (flatten (map W8.w2bits (to_list arr))) ++ w2bits bv ++
+         drop (offset + 32) (flatten (map W8.w2bits (to_list arr))))).
+  rewrite iffE => [#] -> * /=; 1: by smt(in_chunk_size W8.bits2wK).
+  rewrite map_id /= chunkK 1://;1: by rewrite !size_cat size_take;
+    by smt(size_take size_drop  W8.size_w2bits size_cat Array32.size_to_list size_flatten_W8_w2bits size_ge0). 
+  by rewrite !nth_cat !size_cat /=;
+     smt(nth_take nth_drop size_take size_drop  W8.size_w2bits size_cat Array32.size_to_list size_flatten_W8_w2bits size_ge0). 
+rewrite (nth_flatten _ 8); 1: by rewrite allP => i;rewrite mapP => He; elim He;smt(W8.size_w2bits).
+rewrite (nth_map W8.zero []); 1: smt(Array32.size_to_list).
+rewrite nth_mkseq 1:/# /= initiE 1:/# /= /get8 /init8 /set32_direct.
+rewrite initiE 1:/# /=.
+case (offset <= k && k < offset + 32) => *; 1: by 
+  rewrite ifT 1:/#  get_bits8 /= 1,2:/# initiE // initiE //.
+rewrite ifF 1:/# initiE 1:/# /=.
+rewrite (nth_flatten _ 8); 1: by rewrite allP => i;rewrite mapP => He; elim He;smt(W8.size_w2bits).
+rewrite (nth_map W8.zero []); 1: smt(Array32.size_to_list).
+rewrite nth_mkseq 1:/# /= /#. 
+qed.
+
+op sliceset128_8_256 (arr: W8.t Array128.t) (offset: int) (bv: W256.t) : W8.t Array128.t =
+  if 8 %| offset
+  then (init (fun (i3 : int) => get8 (set256_direct ((init8 (fun (i_0 : int) => arr.[i_0])))%WArray128 (offset %/ 8) bv) i3))%Array128
+  else  Array128.of_list witness (map W8.bits2w (chunk 8 (take offset (flatten (map W8.w2bits (to_list arr))) ++ w2bits bv ++
+  drop (offset + 256) (flatten (map W8.w2bits (to_list arr)))))).
+
+bind op [W8.t & W256.t & Array128.t] sliceset128_8_256 "asliceset".
+realize bvaslicesetP. 
+move => arr offset bv H /= k kb; rewrite /sliceset128_8_256 /=. 
+case (8 %| offset) => /= *; last first.
++ rewrite of_listK; 1: by rewrite size_map size_chunk 1:// !size_cat size_take;
+      by smt(size_take size_drop  W8.size_w2bits size_cat Array128.size_to_list size_flatten_W8_w2bits size_ge0). 
+  rewrite -(map_comp W8.w2bits W8.bits2w) /(\o). 
+  have := eq_in_map ((fun (x : bool list) => w2bits ((bits2w x))%W8)) idfun (chunk 8
+        (take offset (flatten (map W8.w2bits (to_list arr))) ++ w2bits bv ++
+         drop (offset + 256) (flatten (map W8.w2bits (to_list arr))))).
+  rewrite iffE => [#] -> * /=; 1: by smt(in_chunk_size W8.bits2wK).
+  rewrite map_id /= chunkK 1://;1: by rewrite !size_cat size_take;
+    by smt(size_take size_drop  W8.size_w2bits size_cat Array128.size_to_list size_flatten_W8_w2bits size_ge0). 
+  by rewrite !nth_cat !size_cat /=;
+     smt(nth_take nth_drop size_take size_drop  W8.size_w2bits size_cat Array128.size_to_list size_flatten_W8_w2bits size_ge0). 
+rewrite (nth_flatten _ 8); 1: by rewrite allP => i;rewrite mapP => He; elim He;smt(W8.size_w2bits).
+rewrite (nth_map W8.zero []); 1: smt(Array128.size_to_list).
+rewrite nth_mkseq 1:/# /= initiE 1:/# /= /get8 /init8 /set256_direct.
+rewrite initiE 1:/# /=.
+case (offset <= k && k < offset + 256) => *; 1: by 
+  rewrite ifT 1:/#  get_bits8 /= 1,2:/# initiE // initiE //.
+rewrite ifF 1:/# initiE 1:/# /=.
+rewrite (nth_flatten _ 8); 1: by rewrite allP => i;rewrite mapP => He; elim He;smt(W8.size_w2bits).
+rewrite (nth_map W8.zero []); 1: smt(Array128.size_to_list).
+rewrite nth_mkseq 1:/# /= /#. 
+qed.
+
+
+op sliceset384_8_256 (arr: W8.t Array384.t) (offset: int) (bv: W256.t) : W8.t Array384.t =
+  if 8 %| offset
+  then (init (fun (i3 : int) => get8 (set256_direct ((init8 (fun (i_0 : int) => arr.[i_0])))%WArray384 (offset %/ 8) bv) i3))%Array384
+  else  Array384.of_list witness (map W8.bits2w (chunk 8 (take offset (flatten (map W8.w2bits (to_list arr))) ++ w2bits bv ++
+  drop (offset + 256) (flatten (map W8.w2bits (to_list arr)))))).
+
+bind op [W8.t & W256.t & Array384.t] sliceset384_8_256 "asliceset".
+realize bvaslicesetP. 
+move => arr offset bv H /= k kb; rewrite /sliceset384_8_256 /=. 
+case (8 %| offset) => /= *; last first.
++ rewrite of_listK; 1: by rewrite size_map size_chunk 1:// !size_cat size_take;
+      by smt(size_take size_drop  W8.size_w2bits size_cat Array384.size_to_list size_flatten_W8_w2bits size_ge0). 
+  rewrite -(map_comp W8.w2bits W8.bits2w) /(\o). 
+  have := eq_in_map ((fun (x : bool list) => w2bits ((bits2w x))%W8)) idfun (chunk 8
+        (take offset (flatten (map W8.w2bits (to_list arr))) ++ w2bits bv ++
+         drop (offset + 256) (flatten (map W8.w2bits (to_list arr))))).
+  rewrite iffE => [#] -> * /=; 1: by smt(in_chunk_size W8.bits2wK).
+  rewrite map_id /= chunkK 1://;1: by rewrite !size_cat size_take;
+    by smt(size_take size_drop  W8.size_w2bits size_cat Array384.size_to_list size_flatten_W8_w2bits size_ge0). 
+  by rewrite !nth_cat !size_cat /=;
+     smt(nth_take nth_drop size_take size_drop  W8.size_w2bits size_cat Array384.size_to_list size_flatten_W8_w2bits size_ge0). 
+rewrite (nth_flatten _ 8); 1: by rewrite allP => i;rewrite mapP => He; elim He;smt(W8.size_w2bits).
+rewrite (nth_map W8.zero []); 1: smt(Array384.size_to_list).
+rewrite nth_mkseq 1:/# /= initiE 1:/# /= /get8 /init8 /set256_direct.
+rewrite initiE 1:/# /=.
+case (offset <= k && k < offset + 256) => *; 1: by 
+  rewrite ifT 1:/#  get_bits8 /= 1,2:/# initiE // initiE //.
+rewrite ifF 1:/# initiE 1:/# /=.
+rewrite (nth_flatten _ 8); 1: by rewrite allP => i;rewrite mapP => He; elim He;smt(W8.size_w2bits).
+rewrite (nth_map W8.zero []); 1: smt(Array384.size_to_list).
+rewrite nth_mkseq 1:/# /= /#. 
+qed.
+
+
+
+op sliceget384_8_256 (arr: W8.t Array384.t) (offset: int) : W256.t = 
+if 8 %| offset then 
+    get256_direct (WArray384.init8 (fun (i_0 : int) => arr.[i_0])) (offset %/ 8)
+   else W256.bits2w (take 256 (drop offset (flatten (map W8.w2bits (to_list arr))))).
+
+bind op [W8.t & W256.t & Array384.t] sliceget384_8_256 "asliceget".
+realize bvaslicegetP.
+move => /= arr offset; rewrite /sliceget384_8_256 /= => H k kb. 
+case (8%| offset) => /= *; last by smt(W256.get_bits2w).
+rewrite /get256_direct pack32E initiE 1:/# /= initiE 1:/# /= initiE 1:/# /=. 
+rewrite nth_take 1,2:/# nth_drop 1,2:/#.
+rewrite (BitEncoding.BitChunking.nth_flatten false 8 _). 
++ rewrite allP => x /=; rewrite mapP => He; elim He;smt(W8.size_w2bits).
+rewrite (nth_map W8.zero []); 1: smt(Array384.size_to_list).
+by rewrite nth_mkseq /#.
+qed.
+
 op sliceget768_16_256 (arr: W16.t Array768.t) (offset: int) : W256.t =
 if 8 %| offset then 
     get256_direct (WArray1536.init16 (fun (i_0 : int) => arr.[i_0])) (offset %/ 8)
@@ -1120,14 +1778,6 @@ op sliceset960_8_128 (arr: W8.t Array960.t) (offset: int) (bv: W128.t) : W8.t Ar
   then Array960.init (fun (i3 : int) => get8 (set128_direct ((init8 (fun (i_0 : int) => arr.[i_0])))%WArray960 (offset %/ 8) bv) i3)
   else  Array960.of_list witness (map W8.bits2w (chunk 8 (take offset (flatten (map W8.w2bits (to_list arr))) ++ w2bits bv ++
   drop (offset + 128) (flatten (map W8.w2bits (to_list arr)))))).
-
-lemma size_flatten_W8_w2bits (a : W8.t list) :
-  (size (flatten (map W8.w2bits (a))))  =  8 * size a.
-proof.
-  rewrite size_flatten -map_comp /(\o) /=.
-  rewrite StdBigop.Bigint.sumzE /= StdBigop.Bigint.BIA.big_mapT /(\o) /=. 
-  rewrite StdBigop.Bigint.big_constz count_predT /#.
-qed.
 
 bind op [W8.t & W128.t & Array960.t] sliceset960_8_128 "asliceset".
 realize bvaslicesetP.
@@ -1153,6 +1803,143 @@ case (offset <= k && k < offset + 128) => *; 1: by
 rewrite ifF 1:/# initiE 1:/# /=.
 rewrite (nth_flatten _ 8); 1: by rewrite allP => i;rewrite mapP => He; elim He;smt(W8.size_w2bits).
 rewrite (nth_map W8.zero []); 1: smt(Array960.size_to_list).
+rewrite nth_mkseq /#.
+qed.
+
+op sliceset160_8_128 (arr: W8.t Array160.t) (offset: int) (bv: W128.t) : W8.t Array160.t = 
+  if 8 %| offset
+  then Array160.init (fun (i3 : int) => get8 (set128_direct ((init8 (fun (i_0 : int) => arr.[i_0])))%WArray160 (offset %/ 8) bv) i3)
+  else  Array160.of_list witness (map W8.bits2w (chunk 8 (take offset (flatten (map W8.w2bits (to_list arr))) ++ w2bits bv ++
+  drop (offset + 128) (flatten (map W8.w2bits (to_list arr)))))).
+
+
+bind op [W8.t & W128.t & Array160.t] sliceset160_8_128 "asliceset".
+realize bvaslicesetP.
+move => arr offset bv H /= k kb; rewrite /sliceset160_8_128 /=. 
+case (8 %| offset) => /= *; last first.
++ rewrite of_listK; 1: by  rewrite size_map size_chunk 1:// !size_cat size_take; 
+      by smt(size_take size_drop  W8.size_w2bits size_cat Array160.size_to_list size_flatten_W8_w2bits size_ge0). 
+  rewrite -(map_comp W8.w2bits W8.bits2w) /(\o). 
+  have := eq_in_map ((fun (x : bool list) => w2bits ((bits2w x))%W8)) idfun (chunk 8
+        (take offset (flatten (map W8.w2bits (to_list arr))) ++ w2bits bv ++
+         drop (offset + 128) (flatten (map W8.w2bits (to_list arr))))).
+  rewrite iffE => [#] -> * /=; 1: by smt(in_chunk_size W8.bits2wK).
+  rewrite map_id /= chunkK 1://;1: by rewrite !size_cat size_take;
+    by smt(size_take size_drop  W8.size_w2bits size_cat Array160.size_to_list size_flatten_W8_w2bits size_ge0). 
+  by rewrite !nth_cat !size_cat /=;
+     smt(nth_take nth_drop size_take size_drop  W8.size_w2bits size_cat Array160.size_to_list size_flatten_W8_w2bits size_ge0). 
+rewrite (nth_flatten _ 8); 1: by rewrite allP => i;rewrite mapP => He; elim He;smt(W8.size_w2bits).
+rewrite (nth_map W8.zero []); 1: smt(Array160.size_to_list).
+rewrite nth_mkseq 1:/# /= initiE 1:/# /= /get8 /set128_direct.
+rewrite initiE 1:/# /=.
+case (offset <= k && k < offset + 128) => *; 1: by 
+  rewrite ifT 1:/#  get_bits8 /= 1,2:/# initiE // initiE //.
+rewrite ifF 1:/# initiE 1:/# /=.
+rewrite (nth_flatten _ 8); 1: by rewrite allP => i;rewrite mapP => He; elim He;smt(W8.size_w2bits).
+rewrite (nth_map W8.zero []); 1: smt(Array160.size_to_list).
+rewrite nth_mkseq /#.
+qed.
+
+
+op sliceset160_8_32 (arr: W8.t Array160.t) (offset: int) (bv: W32.t) : W8.t Array160.t = 
+  if 8 %| offset
+  then Array160.init (fun (i3 : int) => get8 (set32_direct ((init8 (fun (i_0 : int) => arr.[i_0])))%WArray160 (offset %/ 8) bv) i3)
+  else  Array160.of_list witness (map W8.bits2w (chunk 8 (take offset (flatten (map W8.w2bits (to_list arr))) ++ w2bits bv ++
+  drop (offset + 32) (flatten (map W8.w2bits (to_list arr)))))).
+
+
+bind op [W8.t & W32.t & Array160.t] sliceset160_8_32 "asliceset".
+realize bvaslicesetP.
+move => arr offset bv H /= k kb; rewrite /sliceset160_8_32 /=. 
+case (8 %| offset) => /= *; last first.
++ rewrite of_listK; 1: by  rewrite size_map size_chunk 1:// !size_cat size_take; 
+      by smt(size_take size_drop  W8.size_w2bits size_cat Array160.size_to_list size_flatten_W8_w2bits size_ge0). 
+  rewrite -(map_comp W8.w2bits W8.bits2w) /(\o). 
+  have := eq_in_map ((fun (x : bool list) => w2bits ((bits2w x))%W8)) idfun (chunk 8
+        (take offset (flatten (map W8.w2bits (to_list arr))) ++ w2bits bv ++
+         drop (offset + 32) (flatten (map W8.w2bits (to_list arr))))).
+  rewrite iffE => [#] -> * /=; 1: by smt(in_chunk_size W8.bits2wK).
+  rewrite map_id /= chunkK 1://;1: by rewrite !size_cat size_take;
+    by smt(size_take size_drop  W8.size_w2bits size_cat Array160.size_to_list size_flatten_W8_w2bits size_ge0). 
+  by rewrite !nth_cat !size_cat /=;
+     smt(nth_take nth_drop size_take size_drop  W8.size_w2bits size_cat Array160.size_to_list size_flatten_W8_w2bits size_ge0). 
+rewrite (nth_flatten _ 8); 1: by rewrite allP => i;rewrite mapP => He; elim He;smt(W8.size_w2bits).
+rewrite (nth_map W8.zero []); 1: smt(Array160.size_to_list).
+rewrite nth_mkseq 1:/# /= initiE 1:/# /= /get8 /set32_direct.
+rewrite initiE 1:/# /=.
+case (offset <= k && k < offset + 32) => *; 1: by 
+  rewrite ifT 1:/#  get_bits8 /= 1,2:/# initiE // initiE //.
+rewrite ifF 1:/# initiE 1:/# /=.
+rewrite (nth_flatten _ 8); 1: by rewrite allP => i;rewrite mapP => He; elim He;smt(W8.size_w2bits).
+rewrite (nth_map W8.zero []); 1: smt(Array160.size_to_list).
+rewrite nth_mkseq /#.
+qed.
+
+op sliceset1410_8_128 (arr: W8.t Array1410.t) (offset: int) (bv: W128.t) : W8.t Array1410.t = 
+  if 8 %| offset
+  then Array1410.init (fun (i3 : int) => get8 (set128_direct ((init8 (fun (i_0 : int) => arr.[i_0])))%WArray1410 (offset %/ 8) bv) i3)
+  else  Array1410.of_list witness (map W8.bits2w (chunk 8 (take offset (flatten (map W8.w2bits (to_list arr))) ++ w2bits bv ++
+  drop (offset + 128) (flatten (map W8.w2bits (to_list arr)))))).
+
+
+bind op [W8.t & W128.t & Array1410.t] sliceset1410_8_128 "asliceset".
+realize bvaslicesetP.
+move => arr offset bv H /= k kb; rewrite /sliceset1410_8_128 /=. 
+case (8 %| offset) => /= *; last first.
++ rewrite of_listK; 1: by  rewrite size_map size_chunk 1:// !size_cat size_take; 
+      by smt(size_take size_drop  W8.size_w2bits size_cat Array1410.size_to_list size_flatten_W8_w2bits size_ge0). 
+  rewrite -(map_comp W8.w2bits W8.bits2w) /(\o). 
+  have := eq_in_map ((fun (x : bool list) => w2bits ((bits2w x))%W8)) idfun (chunk 8
+        (take offset (flatten (map W8.w2bits (to_list arr))) ++ w2bits bv ++
+         drop (offset + 128) (flatten (map W8.w2bits (to_list arr))))).
+  rewrite iffE => [#] -> * /=; 1: by smt(in_chunk_size W8.bits2wK).
+  rewrite map_id /= chunkK 1://;1: by rewrite !size_cat size_take;
+    by smt(size_take size_drop  W8.size_w2bits size_cat Array1410.size_to_list size_flatten_W8_w2bits size_ge0). 
+  by rewrite !nth_cat !size_cat /=;
+     smt(nth_take nth_drop size_take size_drop  W8.size_w2bits size_cat Array1410.size_to_list size_flatten_W8_w2bits size_ge0). 
+rewrite (nth_flatten _ 8); 1: by rewrite allP => i;rewrite mapP => He; elim He;smt(W8.size_w2bits).
+rewrite (nth_map W8.zero []); 1: smt(Array1410.size_to_list).
+rewrite nth_mkseq 1:/# /= initiE 1:/# /= /get8 /set128_direct.
+rewrite initiE 1:/# /=.
+case (offset <= k && k < offset + 128) => *; 1: by 
+  rewrite ifT 1:/#  get_bits8 /= 1,2:/# initiE // initiE //.
+rewrite ifF 1:/# initiE 1:/# /=.
+rewrite (nth_flatten _ 8); 1: by rewrite allP => i;rewrite mapP => He; elim He;smt(W8.size_w2bits).
+rewrite (nth_map W8.zero []); 1: smt(Array1410.size_to_list).
+rewrite nth_mkseq /#.
+qed.
+
+op sliceset1410_8_64 (arr: W8.t Array1410.t) (offset: int) (bv: W64.t) : W8.t Array1410.t = 
+  if 8 %| offset
+  then Array1410.init (fun (i3 : int) => get8 (set64_direct ((init8 (fun (i_0 : int) => arr.[i_0])))%WArray1410 (offset %/ 8) bv) i3)
+  else  Array1410.of_list witness (map W8.bits2w (chunk 8 (take offset (flatten (map W8.w2bits (to_list arr))) ++ w2bits bv ++
+  drop (offset + 64) (flatten (map W8.w2bits (to_list arr)))))).
+
+
+bind op [W8.t & W64.t & Array1410.t] sliceset1410_8_64 "asliceset".
+realize bvaslicesetP.
+move => arr offset bv H /= k kb; rewrite /sliceset1410_8_64 /=. 
+case (8 %| offset) => /= *; last first.
++ rewrite of_listK; 1: by  rewrite size_map size_chunk 1:// !size_cat size_take; 
+      by smt(size_take size_drop  W8.size_w2bits size_cat Array1410.size_to_list size_flatten_W8_w2bits size_ge0). 
+  rewrite -(map_comp W8.w2bits W8.bits2w) /(\o). 
+  have := eq_in_map ((fun (x : bool list) => w2bits ((bits2w x))%W8)) idfun (chunk 8
+        (take offset (flatten (map W8.w2bits (to_list arr))) ++ w2bits bv ++
+         drop (offset + 64) (flatten (map W8.w2bits (to_list arr))))).
+  rewrite iffE => [#] -> * /=; 1: by smt(in_chunk_size W8.bits2wK).
+  rewrite map_id /= chunkK 1://;1: by rewrite !size_cat size_take;
+    by smt(size_take size_drop  W8.size_w2bits size_cat Array1410.size_to_list size_flatten_W8_w2bits size_ge0). 
+  by rewrite !nth_cat !size_cat /=;
+     smt(nth_take nth_drop size_take size_drop  W8.size_w2bits size_cat Array1410.size_to_list size_flatten_W8_w2bits size_ge0). 
+rewrite (nth_flatten _ 8); 1: by rewrite allP => i;rewrite mapP => He; elim He;smt(W8.size_w2bits).
+rewrite (nth_map W8.zero []); 1: smt(Array1410.size_to_list).
+rewrite nth_mkseq 1:/# /= initiE 1:/# /= /get8 /set64_direct.
+rewrite initiE 1:/# /=.
+case (offset <= k && k < offset + 64) => *; 1: by 
+  rewrite ifT 1:/#  get_bits8 /= 1,2:/# initiE // initiE //.
+rewrite ifF 1:/# initiE 1:/# /=.
+rewrite (nth_flatten _ 8); 1: by rewrite allP => i;rewrite mapP => He; elim He;smt(W8.size_w2bits).
+rewrite (nth_map W8.zero []); 1: smt(Array1410.size_to_list).
 rewrite nth_mkseq /#.
 qed.
 
@@ -1194,6 +1981,78 @@ rewrite (nth_map W8.zero []); 1: smt(Array960.size_to_list).
 rewrite nth_mkseq /#.
 qed.
 
+op sliceset768_16_256 (arr: W16.t Array768.t) (offset: int) (bv: W256.t) : W16.t Array768.t = 
+  if 8 %| offset
+  then Array768.init
+     (WArray1536.get16
+        (set256_direct (WArray1536.init16 (fun (i_0 : int) => arr.[i_0])) (
+           offset %/ 8) bv))
+  else  Array768.of_list witness (map W16.bits2w (chunk 16 (take offset (flatten (map W16.w2bits (to_list arr))) ++ w2bits bv ++
+  drop (offset + 256) (flatten (map W16.w2bits (to_list arr)))))).
+
+bind op [W16.t & W256.t & Array768.t] sliceset768_16_256 "asliceset".
+realize bvaslicesetP.
+move => arr offset bv H /= k kb; rewrite /sliceset768_16_256 /=. 
+case (8 %| offset) => /= *; last first.
++ rewrite of_listK; 1: by  rewrite size_map size_chunk 1:// !size_cat size_take; 
+      by smt(size_take size_drop  W16.size_w2bits size_cat Array768.size_to_list size_flatten_W16_w2bits size_ge0). 
+  rewrite -(map_comp W16.w2bits W16.bits2w) /(\o). 
+  have := eq_in_map ((fun (x : bool list) => w2bits ((bits2w x))%W16)) idfun (chunk 16
+        (take offset (flatten (map W16.w2bits (to_list arr))) ++ w2bits bv ++
+         drop (offset + 256) (flatten (map W16.w2bits (to_list arr))))).
+  rewrite iffE => [#] -> * /=; 1: by smt(in_chunk_size W16.bits2wK).
+  rewrite map_id /= chunkK 1://;1: by rewrite !size_cat size_take;
+    by smt(size_take size_drop  W16.size_w2bits size_cat Array768.size_to_list size_flatten_W16_w2bits size_ge0). 
+  by rewrite !nth_cat !size_cat /=;
+     smt(nth_take nth_drop size_take size_drop  W16.size_w2bits size_cat Array768.size_to_list size_flatten_W16_w2bits size_ge0). 
+rewrite (nth_flatten _ 16); 1: by rewrite allP => i;rewrite mapP => He; elim He;smt(W16.size_w2bits).
+rewrite (nth_map W16.zero []); 1: smt(Array768.size_to_list).
+rewrite nth_mkseq 1:/# /= initiE 1:/# /= /get16 /set256_direct /pack2_t.
+rewrite /get16_direct /pack2_t initiE 1:/# /= initiE 1:/# /= initiE 1:/# /=.
+case (offset <= k && k < offset + 256) => *. 
+  by rewrite ifT 1:/#  get_bits8 /= 1,2:/# initiE // initiE //.
+rewrite ifF 1:/# initiE 1:/# /=.
+rewrite (nth_flatten _ 16); 1: by rewrite allP => i;rewrite mapP => He; elim He;smt(W16.size_w2bits).
+rewrite (nth_map W16.zero []); 1: smt(Array768.size_to_list).
+rewrite nth_mkseq 1:/# /= /(\bits8) initiE 1:/# /#. 
+qed.
+
+op sliceset1024_16_256 (arr: W16.t Array1024.t) (offset: int) (bv: W256.t) : W16.t Array1024.t = 
+  if 8 %| offset
+  then Array1024.init
+     (WArray2048.get16
+        (set256_direct (WArray2048.init16 (fun (i_0 : int) => arr.[i_0])) (
+           offset %/ 8) bv))
+  else  Array1024.of_list witness (map W16.bits2w (chunk 16 (take offset (flatten (map W16.w2bits (to_list arr))) ++ w2bits bv ++
+  drop (offset + 256) (flatten (map W16.w2bits (to_list arr)))))).
+
+bind op [W16.t & W256.t & Array1024.t] sliceset1024_16_256 "asliceset".
+realize bvaslicesetP.
+move => arr offset bv H /= k kb; rewrite /sliceset1024_16_256 /=. 
+case (8 %| offset) => /= *; last first.
++ rewrite of_listK; 1: by  rewrite size_map size_chunk 1:// !size_cat size_take; 
+      by smt(size_take size_drop  W16.size_w2bits size_cat Array1024.size_to_list size_flatten_W16_w2bits size_ge0). 
+  rewrite -(map_comp W16.w2bits W16.bits2w) /(\o). 
+  have := eq_in_map ((fun (x : bool list) => w2bits ((bits2w x))%W16)) idfun (chunk 16
+        (take offset (flatten (map W16.w2bits (to_list arr))) ++ w2bits bv ++
+         drop (offset + 256) (flatten (map W16.w2bits (to_list arr))))).
+  rewrite iffE => [#] -> * /=; 1: by smt(in_chunk_size W16.bits2wK).
+  rewrite map_id /= chunkK 1://;1: by rewrite !size_cat size_take;
+    by smt(size_take size_drop  W16.size_w2bits size_cat Array1024.size_to_list size_flatten_W16_w2bits size_ge0). 
+  by rewrite !nth_cat !size_cat /=;
+     smt(nth_take nth_drop size_take size_drop  W16.size_w2bits size_cat Array1024.size_to_list size_flatten_W16_w2bits size_ge0). 
+rewrite (nth_flatten _ 16); 1: by rewrite allP => i;rewrite mapP => He; elim He;smt(W16.size_w2bits).
+rewrite (nth_map W16.zero []); 1: smt(Array1024.size_to_list).
+rewrite nth_mkseq 1:/# /= initiE 1:/# /= /get16 /set256_direct /pack2_t.
+rewrite /get16_direct /pack2_t initiE 1:/# /= initiE 1:/# /= initiE 1:/# /=.
+case (offset <= k && k < offset + 256) => *. 
+  by rewrite ifT 1:/#  get_bits8 /= 1,2:/# initiE // initiE //.
+rewrite ifF 1:/# initiE 1:/# /=.
+rewrite (nth_flatten _ 16); 1: by rewrite allP => i;rewrite mapP => He; elim He;smt(W16.size_w2bits).
+rewrite (nth_map W16.zero []); 1: smt(Array1024.size_to_list).
+rewrite nth_mkseq 1:/# /= /(\bits8) initiE 1:/# /#. 
+qed.
+
 op init_4_32 (f: int -> W32.t) : W32.t Array4.t = Array4.init f.
 
 bind op [W32.t & Array4.t] init_4_32 "ainit".
@@ -1206,16 +2065,15 @@ qed.
 
 
 (* BEGIN BIND CIRCUITS *)
-
 bind circuit VPBROADCAST_16u16 "VPBROADCAST_16u16".
 bind circuit VPBROADCAST_8u32 "VPBROADCAST_8u32".
 bind circuit VPBROADCAST_4u64 "VPBROADCAST_4u64".
 bind circuit VPMADDWD_256 "VPMADDWD_16u16".
 bind circuit VPSLLV_8u32 "VPSLLV_8u32".
-bind circuit VPSRL_4u64 "VPSRL_4u64".
 bind circuit VPSHUFB_256 "VPSHUFB_256".
 bind circuit VEXTRACTI128 "VEXTRACTI128".
-bind circuit VPBLENDW_128 "VPBLEND_8u16".
+bind circuit VPBLENDW_128 "VPBLENDW_128".
+bind circuit BLENDV_16u8 "VPBLENDVB_128".
 bind circuit VPEXTR_32 "VEXTRACTI32_256".
 bind circuit W4u32.VPEXTR_32 "VEXTRACTI32_128".
 bind circuit VPMULH_16u16 "VPMULH_16u16".
@@ -1227,9 +2085,31 @@ bind circuit W32.mulhi "UMULHI_32".
 
 bind circuit VPSHUFD_256 "VPSHUFD_256".
 bind circuit VPERMQ "VPERMQ".
+bind circuit VPERMD "VPERMD".
 bind circuit VPSRL_4u64 "VPSRL_4u64".
 bind circuit VPADD_4u64 "VPADD_4u64".
 bind circuit VPBLENDD_256 "VPBLEND_8u32".
 bind circuit VPSLLV_4u64 "VPSLLV_4u64".
 bind circuit VPSRLV_4u64 "VPSRLV_4u64".
 bind circuit VPSRLDQ_256 "VPSRLDQ_256".
+bind circuit VPSRLV_8u32 "VPSRLV_8u32".
+bind circuit VPSRLV_16u16 "VPSRLV_16u16".
+bind circuit VPSRL_16u16 "VPSRL_16u16".
+bind circuit VPSRA_16u16 "VPSRA_16u16".
+bind circuit VPSLL_16u16 "VPSLL_16u16".
+bind circuit VPSRL_8u32 "VPSRL_8u32".
+bind circuit VPSLL_8u32 "VPSLL_8u32".
+bind circuit VPSLL_4u64 "VPSLL_4u64".
+bind circuit VPINSR_8u16 "VPINSR_8u16".
+bind circuit VPBROADCAST_2u128 "VPBROADCAST_2u128".
+bind circuit VPACKUS_16u16 "VPACKUS_16u16".
+bind circuit VPMADDUBSW_256 "VPMADDUBSW_256".
+bind circuit VPERM2I128 "VPERM2I128".
+bind circuit VPUNPCKL_4u64 "VPUNPCKL_4u64".
+bind circuit VPUNPCKH_4u64 "VPUNPCKH_4u64".
+bind circuit VMOVSLDUP_256 "VMOVSLDUP_256".
+bind circuit VPBLENDW_256 "VPBLENDW_256".
+bind circuit VPACKSS_16u16 "VPACKSS_16u16".
+bind circuit MOVEMASK_32u8 "VPMOVMSKB_u256u32".
+
+
